---
title: "STSCI 7170 Homework 1"
author: "Yen-Lin Chen (yc2253@cornell.edu)"
output: pdf_document
---


```{r setup, include=FALSE}
knitr::opts_chunk$set(echo = TRUE)
```



## 1.a

Suppose a quadratic form 

$$x'Ax = \sum_i \sum_j x_i a_{ij} x_j = \sum_{i} x_i^2a_{ii} + \sum_{i\neq j}x_ia_{ij}x_j$$ 
where $A \in \mathbb{R}^n$ is an arbitrary matrix therefore $a_{ij} \neq a_{ji}$. We can construct another matrix $A^*$ with $a_{ii}^* = a_{ii}$ and $a_{ij}^* = a_{ji}^* = \frac{1}{2}(a_{ij}+a_{ji})$. As a result, 

$$x'Ax = x'A^*x$$ 
where $A^*$ is a symmetric matrix. 



## 1.b 

Suppose that non-zero $x, y \in \mathbb{R}^n$ with $x'y=0$ are linearly dependent, there exist a non-zero scalar $c$ such that $x = cy$. Then $$||x||^2 = x'x = x'(cy) = cx'y = 0$$ which contradict with the assumption. So $x, y$ must be linearly independent. 



## 1.c

$$tr(AB) = \sum_{i=1}^n \sum_{j=1}^m a_{ij}b_{ji} = \sum_{j=1}^m\sum_{i=1}^nb_{ji}a_{ij}=tr(BA)$$



## 1.5

Let $I\in\mathbb{R}^n$ and $v \in \mathbb{R}^n$
$$(I+vv')\left(I - \frac{vv'}{1+v'v} \right) = I + vv' - \frac{vv'}{1+v'v} - \frac{v'v}{1+v'v}vv' = I + vv' - vv' = I$$


## 1.6

$$M=(a-b)I + bJ = (a-b)(I + \frac{b}{a-b}\mathbf{1}\mathbf{1}')$$
using the result in 1.5 and the fact that $a>b$, we can set 

$$v = \sqrt{\frac{b}{a-b}}\mathbf{1}$$

Therefore, 

$$M^{-1} = \frac{1}{a-b}\left(I-\frac{\frac{b}{a-b}\mathbf{1}\mathbf{1}'}{1+\frac{a}{a-b}\mathbf{1}'\mathbf{1}} \right) = \frac{1}{a-b}\left(I - \frac{b\mathbf{1}\mathbf{1}'}{a-b+nb} \right) = \frac{1}{a-b}\left(I-\frac{bJ}{a-b+nb} \right)$$


## 1.9



## 1.10



## 1.13



## 2.2



## 2.3



## 2.12



## 2.16



## 2.17